lOT OF NEW STUFF to hide healthiness conditions and designs behind the scenes
git-svn-id: orca@517

C-verifier/src/Midend-IVL/Isabelle-UTP-Extended/impl/utp_prog_des_more.thy
@@ -9,32 +9,58 @@ section {*More Operators *}
 
 subsection{*Conditional*}
  
-lift_definition pcond_des :: "'\<alpha> cond \<Rightarrow> '\<alpha> prog \<Rightarrow> '\<alpha> prog \<Rightarrow> '\<alpha> prog" ("IF (_)/ THEN (_) ELSE (_) FI") 
+lift_definition pcond_prog :: "'\<alpha> cond \<Rightarrow> '\<alpha> prog \<Rightarrow> '\<alpha> prog \<Rightarrow> '\<alpha> prog" ("IF (_)/ THEN (_) ELSE (_) FI") 
   is "IfD" by (metis ndesign_H1_H3 ndesign_dcond ndesign_form)
     
-declare pcond_des.rep_eq [prog_rep_eq]
+declare pcond_prog.rep_eq [prog_rep_eq]
   
 subsection{*assert and assume*}
 
-abbreviation passume_des :: "'\<alpha> cond \<Rightarrow> '\<alpha> prog"  
-  where "passume_des c \<equiv> (IF c THEN SKIP ELSE magic FI)"
+abbreviation passume_prog :: "'\<alpha> cond \<Rightarrow> '\<alpha> prog"  
+  where "passume_prog c \<equiv> (IF c THEN SKIP ELSE magic FI)"
 
-abbreviation passert_des :: "'\<alpha> upred \<Rightarrow> '\<alpha> prog" 
-  where "passert_des c \<equiv> (IF c THEN SKIP ELSE abort FI)"
+abbreviation passert_prog :: "'\<alpha> upred \<Rightarrow> '\<alpha> prog" 
+  where "passert_prog c \<equiv> (IF c THEN SKIP ELSE abort FI)"
     
 subsection{*Scoping*}
  
-lift_definition pblock_des ::
+lift_definition pblock_prog ::
   "'\<alpha> prog \<Rightarrow> '\<alpha> prog \<Rightarrow> ('\<alpha> des  \<times> '\<alpha>  des \<Rightarrow> '\<alpha> des \<times> '\<alpha> des  \<Rightarrow> '\<alpha> prog) \<Rightarrow>
       ('\<alpha> des  \<times> '\<alpha> des  \<Rightarrow> '\<alpha> des  \<times> '\<alpha> des \<Rightarrow> '\<alpha> prog) \<Rightarrow> '\<alpha> prog" 
 is blockD oops
-  
+
+subsection{*Recursion*}    
+ 
+lift_definition prec_lfp_prog :: "('\<alpha> prog \<Rightarrow> '\<alpha> prog) \<Rightarrow> '\<alpha> prog" 
+  is "ndesign_lfp" 
+  apply (simp)
+  apply (subst (1) normal_design_theory_continuous.LFP_healthy_comp)
+  apply (subst (2) normal_design_theory_continuous.LFP_healthy_comp) 
+  apply (simp add: comp_def H1_H3_commute H1_idem H3_idem Healthy_def ndes_hcond_def)
+  done
+
+lift_definition prec_gfp_prog :: "('\<alpha> prog \<Rightarrow> '\<alpha> prog) \<Rightarrow> '\<alpha> prog" 
+  is "ndesign_gfp" 
+  apply (simp)
+  apply (subst (1) normal_design_theory_continuous.GFP_healthy_comp)
+  apply (subst (2) normal_design_theory_continuous.GFP_healthy_comp) 
+  apply (simp add: comp_def H1_H3_commute H1_idem H3_idem Healthy_def ndes_hcond_def)
+  done
+    
 subsection{*Iterations*}    
     
-lift_definition pwhile_inv_des :: "'\<alpha> cond \<Rightarrow> '\<alpha> cond \<Rightarrow> '\<alpha> prog \<Rightarrow> '\<alpha> prog " ("WHILE (_)/ INVR (_) DO (_) OD")
-  is "While_inv_ndes" unfolding While_inv_ndes_def While_lfp_ndes_def
+lift_definition pwhile_prog :: "'\<alpha> cond \<Rightarrow>  '\<alpha> prog \<Rightarrow> '\<alpha> prog " ("WHILE (_)/ DO (_) OD")
+  is "While_bot_ndes" unfolding While_lfp_ndes_def
   by simp
+
+definition pwhile_inv_prog :: "'\<alpha> cond \<Rightarrow> '\<alpha> cond \<Rightarrow> '\<alpha> prog \<Rightarrow> '\<alpha> prog " ("INVR (_)/ WHILE (_)/ DO (_) OD")   
+where "INVR I WHILE b DO P OD = WHILE b DO P OD"  
+
+definition pwhile_inv_vrt_prog :: "'\<alpha> cond \<Rightarrow>  ('t,'\<alpha>) uexpr \<Rightarrow> '\<alpha> cond  \<Rightarrow>'\<alpha> prog \<Rightarrow> '\<alpha> prog " ("INVR (_)/ VRT (_)/ WHILE (_)/ DO (_) OD")   
+  where "INVR I VRT E WHILE b DO P OD = WHILE b DO P OD"
     
-declare pwhile_inv_des.rep_eq [prog_rep_eq]
+declare pwhile_prog.rep_eq [prog_rep_eq]
+declare pwhile_inv_prog_def [prog_rep_eq]
+declare pwhile_inv_vrt_prog_def [prog_rep_eq]
  
 end
