C-verifier/src/Midend-IVL/Isabelle-UTP-Extended/hoare/AlgebraicLaws/Abrupt/algebraic_laws_abrupt.thy
@@ -2,6 +2,7 @@ section \<open>Algebraic laws for abrupt designs\<close>
 
 theory algebraic_laws_abrupt
   imports algebraic_laws_abrupt_aux
+          "../Design/Algebraic_laws_design"
 begin
 
 (* TODO: add laws for assigns when composed with try catch... *)
@@ -11,72 +12,69 @@ declare urel_cond [uabr_cond]
 
 subsection Throw
 
-lemma throw_cpa_left_zero_true_abr[uabr_comp]:
+lemma throw_abr_left_zero_true_abr[uabr_comp]:
   "(THROW\<^sub>A\<^sub>B\<^sub>R;; true) = (true)"
   by rel_auto
 
-lemma throw_cpa_left_zero_true_lift_abr[uabr_comp]:
+lemma throw_abr_left_zero_true_lift_abr[uabr_comp]:
   "(THROW\<^sub>A\<^sub>B\<^sub>R;; \<lceil>true\<rceil>\<^sub>A\<^sub>B\<^sub>R) = (\<lceil>true\<rceil>\<^sub>A\<^sub>B\<^sub>R)"
   by rel_auto
 
-lemma throw_cpa_left_zero_false_lift_abr[uabr_comp]:
+lemma throw_abr_left_zero_false_lift_abr[uabr_comp]:
   "(THROW\<^sub>A\<^sub>B\<^sub>R;; \<lceil>false\<rceil>\<^sub>A\<^sub>B\<^sub>R) = (\<lceil>false\<rceil>\<^sub>A\<^sub>B\<^sub>R)"
   by rel_auto
 
-lemma throw_cpa_left_zero_skip_abr[uabr_comp]:
+lemma throw_abr_left_zero_skip_abr[uabr_comp]:
   "(THROW\<^sub>A\<^sub>B\<^sub>R;; SKIP\<^sub>A\<^sub>B\<^sub>R) = (THROW\<^sub>A\<^sub>B\<^sub>R)"
   by rel_auto
 
-lemma throw_cpa_left_zero_assigns_abr[uabr_comp]:
+lemma throw_abr_left_zero_assigns_abr[uabr_comp]:
   "(THROW\<^sub>A\<^sub>B\<^sub>R;; \<langle>\<sigma>\<rangle>\<^sub>A\<^sub>B\<^sub>R) = (THROW\<^sub>A\<^sub>B\<^sub>R)"
   by rel_auto
 
-(*lemma throw_cpa_left_zero_top_abr[uabr_comp]:
+lemma throw_abr_left_unit_top_abr[uabr_comp]:
   "(THROW\<^sub>A\<^sub>B\<^sub>R;; \<top>\<^sub>A\<^sub>B\<^sub>R) = (\<top>\<^sub>A\<^sub>B\<^sub>R)"
-  by rel_auto*)
-
-lemma not_abrupt_left_zero_throw_abr[uabr_comp]:
-  "(($x);; THROW\<^sub>A\<^sub>B\<^sub>R) = ($x)"
   by rel_auto
 
-lemma abrupt_left_zero_throw_abr[uabr_comp]:
-  "($aburpt;; THROW\<^sub>A\<^sub>B\<^sub>R) = $aburpt"
+lemma throw_abr_idem [uabr_comp]:
+  "(THROW\<^sub>A\<^sub>B\<^sub>R;; THROW\<^sub>A\<^sub>B\<^sub>R) = THROW\<^sub>A\<^sub>B\<^sub>R"
+  by rel_auto
+ 
+lemma throw_abr_simpl_abr [uabr_comp]:
+  "(THROW\<^sub>A\<^sub>B\<^sub>R;; Simpl\<^sub>A\<^sub>B\<^sub>R P) = THROW\<^sub>A\<^sub>B\<^sub>R"
+  by rel_auto  
+    
+lemma not_abrupt_left_zero_throw_abr[uabr_comp]:
+  "(($x);; THROW\<^sub>A\<^sub>B\<^sub>R) = ($x)"
   by rel_auto
 
 lemma bot_left_zero_throw_abr[uabr_comp]:
   "(\<top>\<^sub>A\<^sub>B\<^sub>R;; THROW\<^sub>A\<^sub>B\<^sub>R) = (\<top>\<^sub>A\<^sub>B\<^sub>R)"
   by rel_auto
 
-lemma throw_abr_idem [uabr_comp]:
-  "(THROW\<^sub>A\<^sub>B\<^sub>R;; THROW\<^sub>A\<^sub>B\<^sub>R) = THROW\<^sub>A\<^sub>B\<^sub>R"
-  by rel_auto
 
 lemma throw_abr_right_zero_skip_abr[uabr_comp]:
-  "(SKIP\<^sub>A\<^sub>B\<^sub>R;; THROW\<^sub>A\<^sub>B\<^sub>R) = THROW\<^sub>A\<^sub>B\<^sub>R"
-  by rel_auto
-
-(*lemma assigns_abr_throw_abr_right[uabr_comp]:
-  "\<langle>\<sigma>\<rangle>\<^sub>A\<^sub>B\<^sub>R;; THROW\<^sub>A\<^sub>B\<^sub>R = (C3_abr(\<lceil>true\<rceil>\<^sub>A\<^sub>B\<^sub>R \<turnstile> ($abrupt\<acute> \<and> \<lceil>\<langle>\<sigma>\<rangle>\<^sub>a\<rceil>\<^sub>A\<^sub>B\<^sub>R)))"
+  "(SKIP\<^sub>A\<^sub>B\<^sub>R ;; THROW\<^sub>A\<^sub>B\<^sub>R) = THROW\<^sub>A\<^sub>B\<^sub>R"
   by rel_auto
 
 lemma assigns_abr_throw_abr_right[uabr_comp]:
-  "\<langle>\<sigma>\<rangle>\<^sub>A\<^sub>B\<^sub>R;; THROW\<^sub>A\<^sub>B\<^sub>R = (C3_abr(\<lceil>\<sigma>\<rceil>\<^sub>s\<^sub>A\<^sub>B\<^sub>R \<dagger> (\<lceil>true\<rceil>\<^sub>A\<^sub>B\<^sub>R \<turnstile> ($abrupt\<acute> \<and> \<lceil>II\<rceil>\<^sub>A\<^sub>B\<^sub>R))))"
-  by rel_auto*)
+  "\<langle>\<sigma>\<rangle>\<^sub>A\<^sub>B\<^sub>R;; THROW\<^sub>A\<^sub>B\<^sub>R = Simpl\<^sub>A\<^sub>B\<^sub>R(\<lceil>\<sigma>\<rceil>\<^sub>s\<^sub>A\<^sub>B\<^sub>R \<dagger>($abrupt\<acute> \<and> \<lceil>II\<rceil>\<^sub>A\<^sub>B\<^sub>R))"
+  by rel_auto
 
 subsection Skip
 
 text \<open>In this section we introduce the algebraic laws of programming related to the SKIP
       statement.\<close>
 
-lemma true_left_zero_skip_cpa_abr[uabr_comp]:
+lemma true_right_zero_skip_cpa_abr[uabr_comp]:
   "(SKIP\<^sub>A\<^sub>B\<^sub>R;; true) = (true)"
   by rel_auto
 
-lemma true_lift_abr_left_zero_skip_abr[uabr_comp]:
+lemma true_lift_abr_right_zero_skip_abr[uabr_comp]:
   "(SKIP\<^sub>A\<^sub>B\<^sub>R;; \<lceil>true\<rceil>\<^sub>A\<^sub>B\<^sub>R) = (\<lceil>true\<rceil>\<^sub>A\<^sub>B\<^sub>R)"
   by rel_auto
 
-lemma false_lift_abr_left_zero_skip_abr[uabr_comp]:
+lemma false_lift_abr_right_zero_skip_abr[uabr_comp]:
   "(SKIP\<^sub>A\<^sub>B\<^sub>R;; \<lceil>false\<rceil>\<^sub>A\<^sub>B\<^sub>R) = (\<lceil>false\<rceil>\<^sub>A\<^sub>B\<^sub>R)"
   by rel_auto
 
@@ -84,7 +82,7 @@ lemma skip_abr_left_unit_assigns_abr[uabr_comp]:
   "(SKIP\<^sub>A\<^sub>B\<^sub>R;; \<langle>\<sigma>\<rangle>\<^sub>A\<^sub>B\<^sub>R) = (\<langle>\<sigma>\<rangle>\<^sub>A\<^sub>B\<^sub>R)"
   by rel_auto
 
-lemma skip_abr_top_abr_left_zero[uabr_comp]:
+lemma top_abr_right_zero_skip_abr_[uabr_comp]:
   "(SKIP\<^sub>A\<^sub>B\<^sub>R;; \<top>\<^sub>A\<^sub>B\<^sub>R) = (\<top>\<^sub>A\<^sub>B\<^sub>R)"
   by rel_auto
 
@@ -92,7 +90,7 @@ lemma skip_abr_abrupt_left_zero[uabr_comp]:
   "($x;; SKIP\<^sub>A\<^sub>B\<^sub>R) = $x"
   by rel_auto
 
-lemma skip_abr_bot_left_zero[uabr_comp]:
+lemma bot_left_zero_skip_abr[uabr_comp]:
   "(\<top>\<^sub>A\<^sub>B\<^sub>R;; SKIP\<^sub>A\<^sub>B\<^sub>R) = (\<top>\<^sub>A\<^sub>B\<^sub>R)"
   by rel_auto
 
@@ -109,7 +107,7 @@ lemma simpl_pre_skip_abr_post:
   by rel_auto
 
 lemma simpl_pre_skip_abr_var:
-  fixes x :: "(bool \<Longrightarrow> 'b cpa)"
+  fixes x :: "(bool \<Longrightarrow> 'b abr_des)"
   shows "(Simpl\<^sub>A\<^sub>B\<^sub>R $x \<and> SKIP\<^sub>A\<^sub>B\<^sub>R) = (SKIP\<^sub>A\<^sub>B\<^sub>R \<and> Simpl\<^sub>A\<^sub>B\<^sub>R $x\<acute>)"
   by rel_auto
 
@@ -188,13 +186,6 @@ lemma not_abrupt_left_assigns_abr_post_des[urel_cond]:
   apply rel_simp 
 done
 
-lemma  not_abrupt_left_throw_abr_post_des[urel_cond]:
-  "R \<triangleleft> \<not> $abrupt \<triangleright> (S \<turnstile> (THROW\<^sub>A\<^sub>B\<^sub>R;; P))  =
-   R \<triangleleft> \<not> $abrupt \<triangleright> (S \<turnstile> ((\<not>$abrupt) \<turnstile> (\<lceil>II\<rceil>\<^sub>A\<^sub>B\<^sub>R \<and> $abrupt\<acute>));; P)"
-  unfolding assigns_abr_def
-  apply pred_simp
-  apply rel_simp
-done
 
 lemma usubst_abr_cancel [usubst]:
   assumes 1:"weak_lens v"
@@ -214,285 +205,424 @@ lemma assigns_abr_id [uabr_simpl]: "SKIP\<^sub>A\<^sub>B\<^sub>R = \<langle>id\<
 
 lemma assign_test[uabr_comp]:
   assumes 1:"mwb_lens x"
-  shows     "(x \<Midarrow> \<guillemotleft>u\<guillemotright>;; x \<Midarrow> \<guillemotleft>v\<guillemotright>) = (x \<Midarrow> \<guillemotleft>v\<guillemotright>)"
+  shows     "(x :=\<^sub>A\<^sub>B\<^sub>R \<guillemotleft>u\<guillemotright>;; x :=\<^sub>A\<^sub>B\<^sub>R \<guillemotleft>v\<guillemotright>) = (x :=\<^sub>A\<^sub>B\<^sub>R \<guillemotleft>v\<guillemotright>)"
   using 1
   by (simp add: usubst uabr_comp)
 
 lemma assign_abr_left_comp_subst[uabr_comp]:
-  "(x \<Midarrow> u;; Simpl\<^sub>A\<^sub>B\<^sub>R(\<lceil>P\<rceil>\<^sub>A\<^sub>B\<^sub>R \<turnstile> \<lceil>Q\<rceil>\<^sub>A\<^sub>B\<^sub>R)) = Simpl\<^sub>A\<^sub>B\<^sub>R(\<lceil>P\<lbrakk>\<lceil>u\<rceil>\<^sub></$x\<rbrakk>\<rceil>\<^sub>A\<^sub>B\<^sub>R \<turnstile> \<lceil>Q\<lbrakk>\<lceil>u\<rceil>\<^sub></$x\<rbrakk>\<rceil>\<^sub>A\<^sub>B\<^sub>R)"
-  by (simp add: uabr_comp usubst)
+  "(x :=\<^sub>A\<^sub>B\<^sub>R u;; Simpl\<^sub>A\<^sub>B\<^sub>R(\<lceil>P\<rceil>\<^sub>A\<^sub>B\<^sub>R \<turnstile> \<lceil>Q\<rceil>\<^sub>A\<^sub>B\<^sub>R)) = Simpl\<^sub>A\<^sub>B\<^sub>R(\<lceil>P\<lbrakk>\<lceil>u\<rceil>\<^sub></$x\<rbrakk>\<rceil>\<^sub>A\<^sub>B\<^sub>R \<turnstile> \<lceil>Q\<lbrakk>\<lceil>u\<rceil>\<^sub></$x\<rbrakk>\<rceil>\<^sub>A\<^sub>B\<^sub>R)"
+  by rel_auto
 
 lemma assign_abr_twice[uabr_comp]:
   assumes "mwb_lens x" and  "x \<sharp> f"
-  shows "(x \<Midarrow> e;; x \<Midarrow> f) = (x \<Midarrow> f)"
+  shows "(x :=\<^sub>A\<^sub>B\<^sub>R e;; x :=\<^sub>A\<^sub>B\<^sub>R f) = (x :=\<^sub>A\<^sub>B\<^sub>R f)"
   using assms
   by (simp add: uabr_comp usubst)
 
 lemma assign_abr_commute:
   assumes "x \<bowtie> y" "x \<sharp> f" "y \<sharp> e"
-  shows "(x \<Midarrow> e;; y \<Midarrow> f) = (y \<Midarrow> f;; x \<Midarrow> e)"
+  shows "(x :=\<^sub>A\<^sub>B\<^sub>R e;; y :=\<^sub>A\<^sub>B\<^sub>R f) = (y :=\<^sub>A\<^sub>B\<^sub>R f;; x :=\<^sub>A\<^sub>B\<^sub>R e)"
   using assms
   by (simp add: uabr_comp usubst usubst_upd_comm)
 
 lemma assign_abr_cond_abr[uabr_comp]: (*needs more laws to be automatic*)
   fixes x :: "('a \<Longrightarrow> '\<alpha>)"
-  shows "(x \<Midarrow> e;; (bif b then Simpl\<^sub>A\<^sub>B\<^sub>R P else Simpl\<^sub>A\<^sub>B\<^sub>R Q eif)) =
-         (bif (b\<lbrakk>e/x\<rbrakk>) then (x \<Midarrow> e;; Simpl\<^sub>A\<^sub>B\<^sub>R P)  else (x \<Midarrow> e;; Simpl\<^sub>A\<^sub>B\<^sub>R Q) eif)"
-  apply (simp add: usubst uabr_comp)
-  apply rel_auto
-done
+  shows "(x :=\<^sub>A\<^sub>B\<^sub>R e;; (bif\<^sub>A\<^sub>B\<^sub>R b then Simpl\<^sub>A\<^sub>B\<^sub>R P else Simpl\<^sub>A\<^sub>B\<^sub>R Q eif)) =
+         (bif\<^sub>A\<^sub>B\<^sub>R (b\<lbrakk>e/x\<rbrakk>) then (x :=\<^sub>A\<^sub>B\<^sub>R e;; Simpl\<^sub>A\<^sub>B\<^sub>R P)  else (x :=\<^sub>A\<^sub>B\<^sub>R e;; Simpl\<^sub>A\<^sub>B\<^sub>R Q) eif)"
+  by rel_auto
 
 lemma assign_c_uop1[uabr_comp]:
   assumes 1: "mwb_lens v"
-  shows "(v \<Midarrow> e1;; v \<Midarrow> (uop F (&v))) = (v \<Midarrow> (uop F e1))"
-  by (simp add: usubst  uabr_comp assms)
+  shows "(v :=\<^sub>A\<^sub>B\<^sub>R e1;; v :=\<^sub>A\<^sub>B\<^sub>R (uop F (&v))) = (v :=\<^sub>A\<^sub>B\<^sub>R (uop F e1))"
+  by (simp add: usubst uabr_comp assms)
 
 lemma assign_c_bop1[uabr_comp]:
   assumes 1: "mwb_lens v" and 2:"v \<sharp> e2"
-  shows "(v \<Midarrow> e1;; v \<Midarrow>(bop bp (&v) e2)) = (v \<Midarrow> (bop bp e1 e2))"
+  shows "(v :=\<^sub>A\<^sub>B\<^sub>R e1;; v :=\<^sub>A\<^sub>B\<^sub>R (bop bp (&v) e2)) = (v :=\<^sub>A\<^sub>B\<^sub>R (bop bp e1 e2))"
   by (simp add: usubst uabr_comp assms)
 
 lemma assign_c_bop2[uabr_comp]:
   assumes 1: "mwb_lens v" and 2:"v \<sharp> e2"
-  shows "(v \<Midarrow> e1;; v \<Midarrow> (bop bp e2 (&v))) = (v \<Midarrow> (bop bp e2 e1))"
+  shows "(v :=\<^sub>A\<^sub>B\<^sub>R e1;; v :=\<^sub>A\<^sub>B\<^sub>R (bop bp e2 (&v))) = (v :=\<^sub>A\<^sub>B\<^sub>R (bop bp e2 e1))"
   by (simp add: usubst uabr_comp assms)
 
 lemma assign_c_trop1[uabr_comp]:
   assumes 1: "mwb_lens v" and 2:"v \<sharp> e2" and 3:"v \<sharp> e3"
-  shows "(v \<Midarrow> e1;; v \<Midarrow> (trop tp (&v) e2 e3)) =
-         (v \<Midarrow> (trop tp e1 e2 e3))"
+  shows "(v :=\<^sub>A\<^sub>B\<^sub>R e1;; v :=\<^sub>A\<^sub>B\<^sub>R (trop tp (&v) e2 e3)) =
+         (v :=\<^sub>A\<^sub>B\<^sub>R (trop tp e1 e2 e3))"
   by (simp add: usubst uabr_comp assms)
 
 lemma assign_c_trop2[uabr_comp]:
   assumes 1: "mwb_lens v" and 2:"v \<sharp> e2" and 3:"v \<sharp> e3"
-  shows "(v \<Midarrow> e1;; v \<Midarrow> (trop tp e2 (&v) e3)) =
-         (v \<Midarrow> (trop tp e2 e1 e3))"
+  shows "(v :=\<^sub>A\<^sub>B\<^sub>R e1;; v :=\<^sub>A\<^sub>B\<^sub>R (trop tp e2 (&v) e3)) =
+         (v :=\<^sub>A\<^sub>B\<^sub>R (trop tp e2 e1 e3))"
   by (simp add: usubst uabr_comp assms)
 
 lemma assign_c_trop3[uabr_comp]:
   assumes 1: "mwb_lens v" and 2:"v \<sharp> e2" and 3:"v \<sharp> e3"
-  shows "(v \<Midarrow> e1;; v \<Midarrow> (trop tp e2 e3 (&v))) =
-         (v \<Midarrow> (trop tp e2 e3 e1))"
+  shows "(v :=\<^sub>A\<^sub>B\<^sub>R e1;; v :=\<^sub>A\<^sub>B\<^sub>R (trop tp e2 e3 (&v))) =
+         (v :=\<^sub>A\<^sub>B\<^sub>R (trop tp e2 e3 e1))"
   by (simp add: usubst uabr_comp assms)
 
 lemma assign_c_qtop1[uabr_comp]:
   assumes 1: "mwb_lens v" and 2:"v \<sharp> e2" and 3:"v \<sharp> e3" and 4:"v \<sharp> e4"
-  shows "(v \<Midarrow> e1;; v \<Midarrow> (qtop tp (&v) e2 e3 e4)) =
-         (v \<Midarrow> (qtop tp e1 e2 e3 e4))"
+  shows "(v :=\<^sub>A\<^sub>B\<^sub>R e1;; v :=\<^sub>A\<^sub>B\<^sub>R (qtop tp (&v) e2 e3 e4)) =
+         (v :=\<^sub>A\<^sub>B\<^sub>R (qtop tp e1 e2 e3 e4))"
   by (simp add: usubst uabr_comp assms)
 
 lemma assign_c_qtop2[uabr_comp]:
   assumes 1: "mwb_lens v" and 2:"v \<sharp> e2" and 3:"v \<sharp> e3" and 4:"v \<sharp> e4"
-  shows "(v \<Midarrow> e1;; v \<Midarrow> (qtop tp e2 (&v) e3 e4)) =
-         (v \<Midarrow> (qtop tp e2 e1 e3 e4))"
+  shows "(v :=\<^sub>A\<^sub>B\<^sub>R e1;; v :=\<^sub>A\<^sub>B\<^sub>R (qtop tp e2 (&v) e3 e4)) =
+         (v :=\<^sub>A\<^sub>B\<^sub>R (qtop tp e2 e1 e3 e4))"
   by (simp add: usubst uabr_comp assms)
 
 lemma assign_c_qtop3[uabr_comp]:
   assumes 1: "mwb_lens v" and 2:"v \<sharp> e2" and 3:"v \<sharp> e3" and 4:"v \<sharp> e4"
-  shows "(v \<Midarrow> e1;; v \<Midarrow> (qtop tp e2 e3 (&v) e4)) =
-         (v \<Midarrow> (qtop tp e2 e3 e1 e4))"
+  shows "(v :=\<^sub>A\<^sub>B\<^sub>R e1;; v :=\<^sub>A\<^sub>B\<^sub>R (qtop tp e2 e3 (&v) e4)) =
+         (v :=\<^sub>A\<^sub>B\<^sub>R (qtop tp e2 e3 e1 e4))"
   by (simp add: usubst uabr_comp assms)
 
 lemma assign_c_qtop4[uabr_comp]:
   assumes 1: "mwb_lens v" and 2:"v \<sharp> e2" and 3:"v \<sharp> e3" and 4:"v \<sharp> e4"
-  shows "(v \<Midarrow> e1;; v \<Midarrow> (qtop tp e2 e3 e4 (&v))) =
-         (v \<Midarrow> (qtop tp e2 e3 e4 e1))"
+  shows "(v :=\<^sub>A\<^sub>B\<^sub>R e1;; v :=\<^sub>A\<^sub>B\<^sub>R (qtop tp e2 e3 e4 (&v))) =
+         (v :=\<^sub>A\<^sub>B\<^sub>R (qtop tp e2 e3 e4 e1))"
   by (simp add: usubst uabr_comp assms)
 
 text \<open>In the sequel we define assignment laws proposed by Hoare\<close>
 
 lemma assign_abr_vwb_skip_abr[uabr_comp]:
   assumes 1: "vwb_lens v"
-  shows "(v \<Midarrow> &v) = SKIP\<^sub>A\<^sub>B\<^sub>R"
+  shows "(v :=\<^sub>A\<^sub>B\<^sub>R &v) = SKIP\<^sub>A\<^sub>B\<^sub>R"
   by (simp add: assms usubst uabr_simpl)
 
 lemma assign_c_simultaneous:
   assumes  1: "vwb_lens var2"
   and      2: "var1 \<bowtie> var2"
-  shows "var1, var2 \<Midarrow> expr, &var2 = var1 \<Midarrow> expr"
+  shows "var1, var2 :=\<^sub>A\<^sub>B\<^sub>R expr, &var2 = var1 :=\<^sub>A\<^sub>B\<^sub>R expr"
   by (simp add: assms usubst_upd_comm usubst)
 
 lemma assign_c_seq[uabr_comp]:
   assumes  1: "vwb_lens var2"
-  shows"(var1 \<Midarrow> expr);; (var2 \<Midarrow> &var2) = (var1 \<Midarrow> expr)"
+  shows"(var1 :=\<^sub>A\<^sub>B\<^sub>R expr);; (var2 :=\<^sub>A\<^sub>B\<^sub>R &var2) = (var1 :=\<^sub>A\<^sub>B\<^sub>R expr)"
   by (simp add: assms usubst uabr_comp)
 
 lemma assign_c_cond_c_uop[uabr_comp]: (*needs more laws to be automatic*)
   assumes 1: "weak_lens v"
-  shows "bif uop F expr then (v \<Midarrow> expr;; Simpl\<^sub>A\<^sub>B\<^sub>R C1) else (v \<Midarrow> expr;; Simpl\<^sub>A\<^sub>B\<^sub>R C2) eif =
-          v \<Midarrow> expr;; bif uop F (&v) then Simpl\<^sub>A\<^sub>B\<^sub>R C1 else Simpl\<^sub>A\<^sub>B\<^sub>R C2 eif"
-  apply (simp add: assms usubst uabr_comp uabr_simpl)
-  apply pred_simp
-  apply rel_simp
-  apply auto
-  apply (metis assms weak_lens.put_get)+
-done
-
+  shows "bif\<^sub>A\<^sub>B\<^sub>R uop F expr then (v :=\<^sub>A\<^sub>B\<^sub>R expr;; Simpl\<^sub>A\<^sub>B\<^sub>R C1) else (v :=\<^sub>A\<^sub>B\<^sub>R expr;; Simpl\<^sub>A\<^sub>B\<^sub>R C2) eif =
+          v :=\<^sub>A\<^sub>B\<^sub>R expr;; bif\<^sub>A\<^sub>B\<^sub>R uop F (&v) then Simpl\<^sub>A\<^sub>B\<^sub>R C1 else Simpl\<^sub>A\<^sub>B\<^sub>R C2 eif"
+   using assms
+   unfolding assigns_abr_def
+   apply (simp only: simpl_abr_comp_semir)
+   apply  pred_simp
+   apply rel_simp
+   done
+     
 lemma assign_c_cond_bop1[uabr_comp]: (*needs more laws to be automatic*)
   assumes 1: "weak_lens v" and 2: "v \<sharp> exp2"
-  shows "bif bop bp expr exp2 then (v \<Midarrow> expr;; Simpl\<^sub>A\<^sub>B\<^sub>R C1) else (v \<Midarrow> expr;; Simpl\<^sub>A\<^sub>B\<^sub>R C2) eif =
-          v \<Midarrow> expr;; bif bop bp (&v) exp2 then Simpl\<^sub>A\<^sub>B\<^sub>R C1 else Simpl\<^sub>A\<^sub>B\<^sub>R C2 eif"
-  apply (simp add: assms usubst uabr_comp uabr_simpl)
-  apply pred_simp
+  shows "bif\<^sub>A\<^sub>B\<^sub>R bop bp expr exp2 then (v :=\<^sub>A\<^sub>B\<^sub>R expr;; Simpl\<^sub>A\<^sub>B\<^sub>R C1) else (v :=\<^sub>A\<^sub>B\<^sub>R expr;; Simpl\<^sub>A\<^sub>B\<^sub>R C2) eif =
+          v :=\<^sub>A\<^sub>B\<^sub>R expr;; bif\<^sub>A\<^sub>B\<^sub>R bop bp (&v) exp2 then Simpl\<^sub>A\<^sub>B\<^sub>R C1 else Simpl\<^sub>A\<^sub>B\<^sub>R C2 eif"
+  using assms
+  unfolding assigns_abr_def
+  apply (simp only: simpl_abr_comp_semir)
+  apply  pred_simp
   apply rel_simp
-  apply auto
-  apply (metis "1" "2" unrest_uexpr.rep_eq weak_lens.put_get)+
-done
+  done
 
 lemma assign_c_cond_bop2[uabr_comp]: (*needs more laws to be automatic*)
   assumes 1: "weak_lens v" and 2: "v \<sharp> exp2"
-  shows "bif bop bp exp2 expr then (v \<Midarrow> expr;; Simpl\<^sub>A\<^sub>B\<^sub>R C1) else (v \<Midarrow> expr;; Simpl\<^sub>A\<^sub>B\<^sub>R C2) eif =
-          v \<Midarrow> expr;; bif bop bp  exp2 (&v) then Simpl\<^sub>A\<^sub>B\<^sub>R C1 else Simpl\<^sub>A\<^sub>B\<^sub>R C2 eif"
-  apply (simp add: assms usubst uabr_comp uabr_simpl)
-  apply pred_simp
+  shows "bif\<^sub>A\<^sub>B\<^sub>R bop bp exp2 expr then (v :=\<^sub>A\<^sub>B\<^sub>R expr;; Simpl\<^sub>A\<^sub>B\<^sub>R C1) else (v :=\<^sub>A\<^sub>B\<^sub>R expr;; Simpl\<^sub>A\<^sub>B\<^sub>R C2) eif =
+          v :=\<^sub>A\<^sub>B\<^sub>R expr;; bif\<^sub>A\<^sub>B\<^sub>R bop bp  exp2 (&v) then Simpl\<^sub>A\<^sub>B\<^sub>R C1 else Simpl\<^sub>A\<^sub>B\<^sub>R C2 eif"
+  using assms
+  unfolding assigns_abr_def
+  apply (simp only: simpl_abr_comp_semir)
+  apply  pred_simp
   apply rel_simp
-  apply auto
-  apply (metis assms unrest_uexpr.rep_eq weak_lens.put_get)+
 done
 
 lemma assign_cond_trop1[uabr_comp]: (*needs more laws to be automatic*)
   assumes 1: "weak_lens v" and 2: "v \<sharp> exp2" and 3: "v \<sharp> exp3"
-  shows "bif trop bp expr exp2 exp3 then (v \<Midarrow> expr;; Simpl\<^sub>A\<^sub>B\<^sub>R C1) else (v \<Midarrow> expr;; Simpl\<^sub>A\<^sub>B\<^sub>R C2) eif =
-         v \<Midarrow> expr;; bif trop bp (&v) exp2 exp3 then Simpl\<^sub>A\<^sub>B\<^sub>R C1 else Simpl\<^sub>A\<^sub>B\<^sub>R C2 eif"
-  apply (simp add: assms usubst uabr_comp uabr_simpl)
-  apply pred_simp
+  shows "bif\<^sub>A\<^sub>B\<^sub>R trop bp expr exp2 exp3 then (v :=\<^sub>A\<^sub>B\<^sub>R expr;; Simpl\<^sub>A\<^sub>B\<^sub>R C1) else (v :=\<^sub>A\<^sub>B\<^sub>R expr;; Simpl\<^sub>A\<^sub>B\<^sub>R C2) eif =
+         v :=\<^sub>A\<^sub>B\<^sub>R expr;; bif\<^sub>A\<^sub>B\<^sub>R trop bp (&v) exp2 exp3 then Simpl\<^sub>A\<^sub>B\<^sub>R C1 else Simpl\<^sub>A\<^sub>B\<^sub>R C2 eif"
+  using assms
+  unfolding assigns_abr_def
+  apply (simp only: simpl_abr_comp_semir)
+  apply  pred_simp
   apply rel_simp
-  apply auto
-  apply (metis assms unrest_uexpr.rep_eq weak_lens.put_get)+
 done
 
 lemma assign_cond_trop2[uabr_comp]: (*needs more laws to be automatic*)
   assumes 1: "weak_lens v" and 2: "v \<sharp> exp2" and 3: "v \<sharp> exp3"
-  shows "bif trop bp exp2 expr exp3 then (v \<Midarrow> expr;; Simpl\<^sub>A\<^sub>B\<^sub>R C1) else (v \<Midarrow> expr;; Simpl\<^sub>A\<^sub>B\<^sub>R C2) eif =
-         v \<Midarrow> expr;; bif trop bp  exp2 (&v) exp3 then Simpl\<^sub>A\<^sub>B\<^sub>R C1 else Simpl\<^sub>A\<^sub>B\<^sub>R C2 eif"
-  apply (simp add: assms usubst uabr_comp uabr_simpl)
-  apply pred_simp
+  shows "bif\<^sub>A\<^sub>B\<^sub>R trop bp exp2 expr exp3 then (v :=\<^sub>A\<^sub>B\<^sub>R expr;; Simpl\<^sub>A\<^sub>B\<^sub>R C1) else (v :=\<^sub>A\<^sub>B\<^sub>R expr;; Simpl\<^sub>A\<^sub>B\<^sub>R C2) eif =
+         v :=\<^sub>A\<^sub>B\<^sub>R expr;; bif\<^sub>A\<^sub>B\<^sub>R trop bp  exp2 (&v) exp3 then Simpl\<^sub>A\<^sub>B\<^sub>R C1 else Simpl\<^sub>A\<^sub>B\<^sub>R C2 eif"
+  using assms
+  unfolding assigns_abr_def
+  apply (simp only: simpl_abr_comp_semir)
+  apply  pred_simp
   apply rel_simp
-  apply auto
-  apply (metis assms unrest_uexpr.rep_eq weak_lens.put_get)+
 done
 
 lemma assign_cond_trop3[uabr_comp]: (*needs more laws to be automatic*)
   assumes 1: "weak_lens v" and 2: "v \<sharp> exp2" and 3: "v \<sharp> exp3"
-  shows "bif trop bp exp2 exp3 expr then (v \<Midarrow> expr;; Simpl\<^sub>A\<^sub>B\<^sub>R C1) else (v \<Midarrow> expr;; Simpl\<^sub>A\<^sub>B\<^sub>R C2) eif =
-         v \<Midarrow> expr;; bif trop bp exp2 exp3 (&v) then Simpl\<^sub>A\<^sub>B\<^sub>R C1 else Simpl\<^sub>A\<^sub>B\<^sub>R C2 eif"
-  apply (simp add: assms usubst uabr_comp uabr_simpl)
-  apply pred_simp
+  shows "bif\<^sub>A\<^sub>B\<^sub>R trop bp exp2 exp3 expr then (v :=\<^sub>A\<^sub>B\<^sub>R expr;; Simpl\<^sub>A\<^sub>B\<^sub>R C1) else (v :=\<^sub>A\<^sub>B\<^sub>R expr;; Simpl\<^sub>A\<^sub>B\<^sub>R C2) eif =
+         v :=\<^sub>A\<^sub>B\<^sub>R expr;; bif\<^sub>A\<^sub>B\<^sub>R trop bp exp2 exp3 (&v) then Simpl\<^sub>A\<^sub>B\<^sub>R C1 else Simpl\<^sub>A\<^sub>B\<^sub>R C2 eif"
+  using assms
+  unfolding assigns_abr_def
+  apply (simp only: simpl_abr_comp_semir)
+  apply  pred_simp
   apply rel_simp
-  apply auto
-  apply (metis assms unrest_uexpr.rep_eq weak_lens.put_get)+
 done
 
 lemma assign_cond_qtop1[uabr_comp]: (*needs more laws to be automatic*)
   assumes 1: "weak_lens v" and 2: "v \<sharp> exp2" and 3: "v \<sharp> exp3" and 4: "v \<sharp> exp4"
-  shows "bif qtop bp expr exp2 exp3 exp4 then (v \<Midarrow> expr;; Simpl\<^sub>A\<^sub>B\<^sub>R C1) else (v \<Midarrow> expr;; Simpl\<^sub>A\<^sub>B\<^sub>R C2) eif =
-         v \<Midarrow> expr;; bif qtop bp (&v) exp2 exp3 exp4 then Simpl\<^sub>A\<^sub>B\<^sub>R C1 else Simpl\<^sub>A\<^sub>B\<^sub>R C2 eif"
-  apply (simp add: assms usubst uabr_comp uabr_simpl)
-  apply pred_simp
+  shows "bif\<^sub>A\<^sub>B\<^sub>R qtop bp expr exp2 exp3 exp4 then (v :=\<^sub>A\<^sub>B\<^sub>R expr;; Simpl\<^sub>A\<^sub>B\<^sub>R C1) else (v :=\<^sub>A\<^sub>B\<^sub>R expr;; Simpl\<^sub>A\<^sub>B\<^sub>R C2) eif =
+         v :=\<^sub>A\<^sub>B\<^sub>R expr;; bif\<^sub>A\<^sub>B\<^sub>R qtop bp (&v) exp2 exp3 exp4 then Simpl\<^sub>A\<^sub>B\<^sub>R C1 else Simpl\<^sub>A\<^sub>B\<^sub>R C2 eif"
+  using assms
+  unfolding assigns_abr_def
+  apply (simp only: simpl_abr_comp_semir)
+  apply  pred_simp
   apply rel_simp
-  apply auto
-  apply (metis assms unrest_uexpr.rep_eq weak_lens.put_get)+
 done
 
 lemma assign_c_cond_qtop2[uabr_comp]: (*needs more laws to be automatic*)
   assumes 1: "weak_lens v" and 2: "v \<sharp> exp2" and 3: "v \<sharp> exp3" and 4:"v \<sharp> exp4"
-  shows "bif qtop bp exp2 expr  exp3 exp4 then (v \<Midarrow> expr;; Simpl\<^sub>A\<^sub>B\<^sub>R C1) else (v \<Midarrow> expr;; Simpl\<^sub>A\<^sub>B\<^sub>R C2) eif =
-         v \<Midarrow> expr;; bif qtop bp exp2 (&v) exp3 exp4 then Simpl\<^sub>A\<^sub>B\<^sub>R C1 else Simpl\<^sub>A\<^sub>B\<^sub>R C2 eif"
-  apply (simp add: assms usubst uabr_comp uabr_simpl)
-  apply pred_simp
+  shows "bif\<^sub>A\<^sub>B\<^sub>R qtop bp exp2 expr  exp3 exp4 then (v :=\<^sub>A\<^sub>B\<^sub>R expr;; Simpl\<^sub>A\<^sub>B\<^sub>R C1) else (v :=\<^sub>A\<^sub>B\<^sub>R expr;; Simpl\<^sub>A\<^sub>B\<^sub>R C2) eif =
+         v :=\<^sub>A\<^sub>B\<^sub>R expr;; bif\<^sub>A\<^sub>B\<^sub>R qtop bp exp2 (&v) exp3 exp4 then Simpl\<^sub>A\<^sub>B\<^sub>R C1 else Simpl\<^sub>A\<^sub>B\<^sub>R C2 eif"
+  using assms
+  unfolding assigns_abr_def
+  apply (simp only: simpl_abr_comp_semir)
+  apply  pred_simp
   apply rel_simp
-  apply auto
-  apply (metis assms unrest_uexpr.rep_eq weak_lens.put_get)+
 done
 
 lemma assign_c_cond_qtop3[uabr_comp]: (*needs more laws to be automatic*)
   assumes 1: "weak_lens v" and 2: "v \<sharp> exp2" and 3: "v \<sharp> exp3" and 4: "v \<sharp> exp4"
-  shows "bif qtop bp exp2 exp3 expr exp4 then (v \<Midarrow> expr;; Simpl\<^sub>A\<^sub>B\<^sub>R C1) else (v \<Midarrow> expr;; Simpl\<^sub>A\<^sub>B\<^sub>R C2) eif =
-         v \<Midarrow> expr;; bif qtop bp exp2 exp3 (&v) exp4 then Simpl\<^sub>A\<^sub>B\<^sub>R C1 else Simpl\<^sub>A\<^sub>B\<^sub>R C2 eif"
-  apply (simp add: assms usubst uabr_comp uabr_simpl)
-  apply pred_simp
+  shows "bif\<^sub>A\<^sub>B\<^sub>R qtop bp exp2 exp3 expr exp4 then (v :=\<^sub>A\<^sub>B\<^sub>R expr;; Simpl\<^sub>A\<^sub>B\<^sub>R C1) else (v :=\<^sub>A\<^sub>B\<^sub>R expr;; Simpl\<^sub>A\<^sub>B\<^sub>R C2) eif =
+         v :=\<^sub>A\<^sub>B\<^sub>R expr;; bif\<^sub>A\<^sub>B\<^sub>R qtop bp exp2 exp3 (&v) exp4 then Simpl\<^sub>A\<^sub>B\<^sub>R C1 else Simpl\<^sub>A\<^sub>B\<^sub>R C2 eif"
+  using assms
+  unfolding assigns_abr_def
+  apply (simp only: simpl_abr_comp_semir)
+  apply  pred_simp
   apply rel_simp
-  apply auto
-  apply (metis assms unrest_uexpr.rep_eq weak_lens.put_get)+
 done
 
 lemma assign_c_cond_qtop4[uabr_comp]: (*needs more laws to be automatic*)
   assumes 1: "weak_lens v" and 2: "v \<sharp> exp2" and 3: "v \<sharp> exp3" and 4: "v \<sharp> exp4"
-  shows "bif qtop bp exp2 exp3 exp4 expr then (v \<Midarrow> expr;; Simpl\<^sub>A\<^sub>B\<^sub>R C1) else (v \<Midarrow> expr;; Simpl\<^sub>A\<^sub>B\<^sub>R C2) eif =
-         v \<Midarrow> expr;; bif qtop bp exp2  exp3 exp4 (&v) then Simpl\<^sub>A\<^sub>B\<^sub>R C1 else Simpl\<^sub>A\<^sub>B\<^sub>R C2 eif"
-  apply (simp add: assms usubst uabr_comp uabr_simpl)
-  apply pred_simp
+  shows "bif\<^sub>A\<^sub>B\<^sub>R qtop bp exp2 exp3 exp4 expr then (v :=\<^sub>A\<^sub>B\<^sub>R expr;; Simpl\<^sub>A\<^sub>B\<^sub>R C1) else (v :=\<^sub>A\<^sub>B\<^sub>R expr;; Simpl\<^sub>A\<^sub>B\<^sub>R C2) eif =
+         v :=\<^sub>A\<^sub>B\<^sub>R expr;; bif\<^sub>A\<^sub>B\<^sub>R qtop bp exp2  exp3 exp4 (&v) then Simpl\<^sub>A\<^sub>B\<^sub>R C1 else Simpl\<^sub>A\<^sub>B\<^sub>R C2 eif"
+  using assms
+  unfolding assigns_abr_def
+  apply (simp only: simpl_abr_comp_semir)
+  apply  pred_simp
   apply rel_simp
-  apply auto
-  apply (metis assms unrest_uexpr.rep_eq weak_lens.put_get)+
 done
 
-lemma assign_c_cond_If [uabr_cond]:
-  "(bif bexp then (v \<Midarrow> exp1) else (v \<Midarrow> exp2) eif) =
-   (v \<Midarrow> (exp1 \<triangleleft> bexp \<triangleright> exp2))"
+lemma assigns_abr_cond_abr [uabr_cond]:
+  "(bif\<^sub>A\<^sub>B\<^sub>R bexp then (v :=\<^sub>A\<^sub>B\<^sub>R exp1) else (v :=\<^sub>A\<^sub>B\<^sub>R exp2) eif) =
+   (v :=\<^sub>A\<^sub>B\<^sub>R (exp1 \<triangleleft> bexp \<triangleright> exp2))"
   by rel_auto
 
-subsection \<open>While laws\<close>
+
+subsection \<open>While laws for designs\<close>
+  
 text \<open>In this section we introduce the algebraic laws of programming related to the while
       statement.\<close>
-
-theorem while_unfold:
-  "while b do P od = (bif b then (P;; while b do P od) else SKIP\<^sub>A\<^sub>B\<^sub>R eif)"
+lemma "mono (\<lambda>X. bif\<^sub>A\<^sub>B\<^sub>R b then (B ;; X) else SKIP\<^sub>A\<^sub>B\<^sub>R eif)"
+  apply (rule monoI)
+  apply (rule cond_mono)
+     apply (rule cond_mono)
+theorem while_abr_des_unfold_gen:
+  assumes HB: "B is H1"
+  shows "while\<^sub>D\<^sub>A\<^sub>B\<^sub>R b do B od = (bif\<^sub>A\<^sub>B\<^sub>R b then (B;;while\<^sub>D\<^sub>A\<^sub>B\<^sub>R b do B od) else SKIP\<^sub>A\<^sub>B\<^sub>R eif)"
 proof -
-  have m:"mono (\<lambda>X. bif b then (P;; X) else SKIP\<^sub>A\<^sub>B\<^sub>R eif)"
-    by (auto intro: monoI seqr_mono if_mono)
-  have "(while b do P od) = (\<nu> X \<bullet> bif b then (P;; X) else SKIP\<^sub>A\<^sub>B\<^sub>R eif)"
-    by (simp add: While_def)
-  also have "... = (bif b then (P;; (\<nu> X \<bullet> bif b then (P;; X) else SKIP\<^sub>A\<^sub>B\<^sub>R eif)) else SKIP\<^sub>A\<^sub>B\<^sub>R eif)"
-    by (subst lfp_unfold,simp_all add:m)
-  also have "... = (bif b then (P;; while b do P od) else SKIP\<^sub>A\<^sub>B\<^sub>R eif)"
-    by (simp add: While_def)
+  have m:"mono (\<lambda>X. bif\<^sub>A\<^sub>B\<^sub>R b then (B ;; X) else SKIP\<^sub>A\<^sub>B\<^sub>R eif)"
+      apply (simp only: cond_mono)
+
+    by (auto intro: monoI seqr_mono cond_mono)
+  have H: "(\<lambda>X. bif\<^sub>D b then (B ;; X) else SKIP\<^sub>D eif) \<in> \<lbrakk>\<^bold>H\<rbrakk>\<^sub>H \<rightarrow> \<lbrakk>\<^bold>H\<rbrakk>\<^sub>H"
+    using HB
+    apply pred_simp apply rel_simp apply smt done       
+  have "(while\<^sub>D b do B od) = (\<mu>\<^sub>D X \<bullet> bif\<^sub>D b then (B ;; X) else SKIP\<^sub>D eif)"
+    by (simp add: While_lfp_des_def)
+  also have "... = (bif\<^sub>D b then (B;; (\<mu>\<^sub>D X \<bullet> bif\<^sub>D b then (B ;; X) else SKIP\<^sub>D eif)) else SKIP\<^sub>D eif)"
+    using mono_Monotone_utp_order [OF m, of "\<H>\<^bsub>DES\<^esub>"] H
+          design_theory_continuous.LFP_weak_unfold 
+    by auto
+  also have "... = (bif\<^sub>D b then (B;; while\<^sub>D b do B od) else SKIP\<^sub>D eif)"
+    by (simp add: While_lfp_des_def)
   finally show ?thesis .
 qed
+     
+lemma while_inv_des_unfold:
+   assumes HB: "B is H1"
+  shows "(while\<^sub>D b invr p  do B od) = 
+   (bif\<^sub>D b then (B ;; (while\<^sub>D b invr p  do B od)) else SKIP\<^sub>D eif)"
+  unfolding While_inv_des_def using while_des_unfold_gen assms
+  by auto
 
-lemma while_true:
-  shows "(while true do (P\<turnstile>Q) od) = false"(*it should eq to \<top>\<^sub>A\<^sub>B\<^sub>R*)
-  apply (simp add: While_def alpha)
+lemma while_inv_vrt_des_unfold:
+   assumes HB: "B is H1"
+  shows "(while\<^sub>D b invr p vrt e do B od) = 
+   (bif\<^sub>D b then (B ;; (while\<^sub>D b invr p vrt e do B od)) else SKIP\<^sub>D eif)"
+  unfolding While_inv_vrt_des_def using while_des_unfold_gen assms
+  by auto
+    
+theorem while_bot_des_true: 
+  "while\<^sub>D true do P od = (\<mu>\<^sub>D X \<bullet> (P ;; X))"
+  by (simp add: While_lfp_des_def alpha)
+
+lemma while_inv_des_true: 
+  "while\<^sub>D true invr p do P od = (\<mu>\<^sub>D X \<bullet> (P ;; X))"
+   unfolding While_inv_des_def using while_bot_des_true
+   by auto    
+
+lemma while_inv_vrt_des_true: 
+  "while\<^sub>D true invr p vrt e do P od = (\<mu>\<^sub>D X \<bullet> (P ;; X))"
+   unfolding While_inv_vrt_des_def using while_bot_des_true
+   by auto 
+     
+lemma while_des_false:
+  shows "(while\<^sub>D false do P od) = SKIP\<^sub>D"
+  by (simp add: While_lfp_des_def alpha skip_d_def 
+      design_theory_continuous.LFP_const rdesign_is_H1_H2)
+
+lemma while_inv_des_false:
+  shows "(while\<^sub>D false invr p do P od) = SKIP\<^sub>D"
+   unfolding While_inv_des_def using while_des_false
+   by auto  
+
+lemma while_inv_vrt_des_false:
+  shows "(while\<^sub>D false invr p vrt e do P od) = SKIP\<^sub>D"
+   unfolding While_inv_vrt_des_def using while_des_false
+   by auto  
+        
+theorem while_top_des_unfold_gen:
+  assumes HB: "B is H1"
+  shows
+  "while\<^sup>\<top>\<^sup>D b do B od = (bif\<^sub>D b then (B ;; while\<^sup>\<top>\<^sup>D b do B od) else SKIP\<^sub>D eif)"
+proof -
+  have m:"mono (\<lambda>X. bif\<^sub>D b then (B ;; X) else SKIP\<^sub>D eif)"
+    by (auto intro: monoI seqr_mono cond_mono)
+  have H: "(\<lambda>X. bif\<^sub>D b then (B ;; X) else SKIP\<^sub>D eif) \<in> \<lbrakk>\<^bold>H\<rbrakk>\<^sub>H \<rightarrow> \<lbrakk>\<^bold>H\<rbrakk>\<^sub>H"  
+    using HB
+    apply pred_simp apply rel_simp apply smt done     
+  have "(while\<^sup>\<top>\<^sup>D b do B od) = (\<nu>\<^sub>D X \<bullet> bif\<^sub>D b then (B;; X) else SKIP\<^sub>D eif)"
+    by (simp add: While_gfp_des_def)
+  also have "... = (bif\<^sub>D b then (B ;; (\<nu>\<^sub>D X \<bullet> bif\<^sub>D b then (B ;; X) else SKIP\<^sub>D eif)) else SKIP\<^sub>D eif)"
+    using mono_Monotone_utp_order [OF m, of "\<H>\<^bsub>DES\<^esub>"] H
+          design_theory_continuous.GFP_weak_unfold 
+    by auto
+  also have "... = (bif\<^sub>D b then (B ;; while\<^sup>\<top>\<^sup>D b do B od) else SKIP\<^sub>D eif)"
+    by (simp add:While_gfp_des_def)
+  finally show ?thesis .
+qed    
+ 
+theorem while_top_des_false: 
+  "while\<^sup>\<top>\<^sup>D false do P od = SKIP\<^sub>D"
+ by (simp add: While_gfp_des_def alpha skip_d_def 
+      design_theory_continuous.GFP_const rdesign_is_H1_H2)
+    
+(*lemma while_true:
+  shows "(while true do (P\<turnstile>Q) od) = false"it should eq to \<top>\<^sub>D
+  apply (simp add: While_lfp_des_def alpha)
    apply (rule antisym)
   apply (simp_all)
   apply (rule lfp_lowerbound)
   apply (simp)
-  done
+  done*)
+
+subsection \<open>While laws for normal designs\<close>
+text \<open>In this section we introduce the algebraic laws of programming related to the while
+      statement.\<close>
+  
+theorem while_bot_ndes_unfold_gen:
+  assumes HB: "B is H1"
+  shows
+  "while\<^sub>N b do B od = (bif\<^sub>D b then (B;; while\<^sub>N b do B od) else SKIP\<^sub>D eif)"
+proof -
+  have m:"mono (\<lambda>X. bif\<^sub>D b then (B ;; X) else SKIP\<^sub>D eif)"
+    by (auto intro: monoI seqr_mono cond_mono)
+  have H: "(\<lambda>X. bif\<^sub>D b then (B ;; X) else SKIP\<^sub>D eif) \<in> \<lbrakk>\<^bold>N\<rbrakk>\<^sub>H \<rightarrow> \<lbrakk>\<^bold>N\<rbrakk>\<^sub>H"
+    using HB apply pred_simp apply rel_simp apply smt done       
+  have "(while\<^sub>N b do B od) = (\<mu>\<^sub>N X \<bullet> bif\<^sub>D b then (B ;; X) else SKIP\<^sub>D eif)"
+    by (simp add: While_lfp_ndes_def)
+  also have "... = (bif\<^sub>D b then (B ;; (\<mu>\<^sub>N X \<bullet> bif\<^sub>D b then (B ;; X) else SKIP\<^sub>D eif)) else SKIP\<^sub>D eif)"
+    using mono_Monotone_utp_order [OF m, of "\<H>\<^bsub>NDES\<^esub>"] H
+          normal_design_theory_continuous.LFP_weak_unfold 
+    by auto
+  also have "... = (bif\<^sub>D b then (B ;; while\<^sub>N b do B od) else SKIP\<^sub>D eif)"
+    by (simp add: While_lfp_ndes_def)
+  finally show ?thesis .
+qed
     
-lemma while_false:
-  shows "(while false do P od) = SKIP\<^sub>A\<^sub>B\<^sub>R"
-proof -
-  have "(while false do P od) = bif false then (P;; while false do P od) else SKIP\<^sub>A\<^sub>B\<^sub>R eif"
-    using while_unfold[of _ P] by simp
-  also have "... = SKIP\<^sub>A\<^sub>B\<^sub>R" by rel_blast
-  finally show ?thesis .
-qed
+lemma while_inv_ndes_unfold:
+  assumes HB: "B is H1"
+  shows
+  "(while\<^sub>N b invr p  do B od) = 
+   (bif\<^sub>D b then (B ;; (while\<^sub>N b invr p  do B od)) else SKIP\<^sub>D eif)"
+  unfolding While_inv_ndes_def using while_bot_ndes_unfold_gen assms
+  by auto  
 
-lemma while_inv_unfold:
-  "(while b invr p do P od) = (bif b then (P ;; (while b invr p do P od)) else SKIP\<^sub>A\<^sub>B\<^sub>R eif)"
-  unfolding While_inv_def using while_unfold
+lemma while_inv_vrt_ndes_unfold:
+  assumes HB: "B is H1"
+  shows
+  "(while\<^sub>N b invr p vrt e do B od) = 
+   (bif\<^sub>D b then (B ;; (while\<^sub>N b invr p vrt e do B od)) else SKIP\<^sub>D eif)"
+  unfolding While_inv_vrt_ndes_def using while_bot_ndes_unfold_gen assms
+  by auto 
+
+theorem while_bot_ndes_true: "while\<^sub>N true do P od = (\<mu>\<^sub>N X \<bullet> (P;; X))"
+  by (simp add: While_lfp_ndes_def alpha)
+        
+lemma while_inv_ndes_true:
+  "(while\<^sub>N true invr p  do B od) = (\<mu>\<^sub>N X \<bullet> (B;; X))"
+  unfolding While_inv_ndes_def using while_bot_ndes_true 
+  by auto 
+
+lemma while_inv_vrt_ndes_true:
+  "(while\<^sub>N true invr p vrt e do B od) = (\<mu>\<^sub>N X \<bullet> (B;; X))"
+  unfolding While_inv_vrt_ndes_def using while_bot_ndes_true 
   by auto
+    
+lemma while_ndes_false:
+  shows "(while\<^sub>N false do P od) = SKIP\<^sub>D"
+  by (simp add: While_lfp_ndes_def alpha skip_d_is_H1_H3  
+      normal_design_theory_continuous.LFP_const)
 
-theorem while_bot_unfold:
-  "while\<^sub>\<bottom> b do P od = (bif b then (P;; while\<^sub>\<bottom> b do P od) else SKIP\<^sub>A\<^sub>B\<^sub>R eif)"
+lemma while_inv_ndes_false:
+  "(while\<^sub>N false invr p  do B od) = SKIP\<^sub>D"
+  unfolding While_inv_ndes_def using while_ndes_false 
+  by auto  
+
+lemma while_inv_vrt_ndes_false:
+  "(while\<^sub>N false invr p vrt e do B od) = SKIP\<^sub>D"
+  unfolding While_inv_vrt_ndes_def using while_ndes_false 
+  by auto 
+          
+theorem while_top_ndes_unfold:
+  assumes HB: "B is H1"
+  shows
+  "while\<^sup>\<top>\<^sup>N b do B od = (bif\<^sub>D b then (B ;; while\<^sup>\<top>\<^sup>N b do B od) else SKIP\<^sub>D eif)"
 proof -
-  have m:"mono (\<lambda>X. bif b then (P;; X) else SKIP\<^sub>A\<^sub>B\<^sub>R eif)"
-    by (auto intro: monoI seqr_mono if_mono)
-  have "(while\<^sub>\<bottom> b do P od) = (\<mu> X \<bullet> bif b then (P;; X) else SKIP\<^sub>A\<^sub>B\<^sub>R eif)"
-    by (simp add: While_bot_def)
-  also have "... = (bif b then (P;; (\<mu> X \<bullet> bif b then (P;; X) else SKIP\<^sub>A\<^sub>B\<^sub>R eif)) else SKIP\<^sub>A\<^sub>B\<^sub>R eif)"
-    by (subst gfp_unfold, simp_all add: m)
-  also have "... = (bif b then (P;; while\<^sub>\<bottom> b do P od) else SKIP\<^sub>A\<^sub>B\<^sub>R eif)"
-    by (simp add: While_bot_def)
+  have m:"mono (\<lambda>X. bif\<^sub>D b then (B ;; X) else SKIP\<^sub>D eif)"
+    by (auto intro: monoI seqr_mono cond_mono)
+  have H: "(\<lambda>X. bif\<^sub>D b then (B ;; X) else SKIP\<^sub>D eif) \<in> \<lbrakk>\<^bold>N\<rbrakk>\<^sub>H \<rightarrow> \<lbrakk>\<^bold>N\<rbrakk>\<^sub>H" 
+    using HB
+    apply pred_simp apply rel_simp apply smt done     
+  have "(while\<^sup>\<top>\<^sup>N b do B od) = (\<nu>\<^sub>N X \<bullet> bif\<^sub>D b then (B;; X) else SKIP\<^sub>D eif)"
+    by (simp add: While_gfp_ndes_def)
+  also have "... = (bif\<^sub>D b then (B ;; (\<nu>\<^sub>N X \<bullet> bif\<^sub>D b then (B ;; X) else SKIP\<^sub>D eif)) else SKIP\<^sub>D eif)"
+    using mono_Monotone_utp_order [OF m, of "\<H>\<^bsub>NDES\<^esub>"] H
+          normal_design_theory_continuous.GFP_weak_unfold 
+    by auto
+  also have "... = (bif\<^sub>D b then (B ;; while\<^sup>\<top>\<^sup>N b do B od) else SKIP\<^sub>D eif)"
+    by (simp add:While_gfp_ndes_def)
   finally show ?thesis .
 qed
 
-theorem while_bot_false: "while\<^sub>\<bottom> false do P od = SKIP\<^sub>A\<^sub>B\<^sub>R"
-  by (simp add: While_bot_def mu_const alpha)
-
-theorem while_bot_true: "while\<^sub>\<bottom> true do P od = (\<mu> X \<bullet> (P;; X))"
-  by (simp add: While_bot_def alpha)
-
+theorem while_bot_ndes_false: "while\<^sup>\<top>\<^sup>N false do B od = SKIP\<^sub>D"
+ by (simp add: While_gfp_ndes_def alpha skip_d_is_H1_H3  
+      normal_design_theory_continuous.GFP_const)
+    
 subsection \<open>assume laws\<close>
 
 lemma assume_twice[uabr_comp]: "(b\<^sup>\<top>\<^sup>C;; c\<^sup>\<top>\<^sup>C) = (b \<and> c)\<^sup>\<top>\<^sup>C"
