C-verifier/src/Midend-IVL/Isabelle-UTP-Extended/hoare/AlgebraicLaws/Abrupt/algebraic_laws_abrupt_aux.thy
@@ -60,42 +60,34 @@ lemma rel_usubst_lift_cpa_in_out_abrupt_ok[usubst]:
   "\<lceil>\<sigma>\<rceil>\<^sub>S\<^sub>A\<^sub>B\<^sub>R \<dagger> ($abrupt\<acute>) = (($abrupt\<acute>))" "\<lceil>\<sigma>\<rceil>\<^sub>S\<^sub>A\<^sub>B\<^sub>R \<dagger> (\<not>$abrupt\<acute>) = (\<not>$abrupt\<acute>)"
   "\<lceil>\<sigma>\<rceil>\<^sub>S\<^sub>A\<^sub>B\<^sub>R \<dagger> ($ok\<acute>) = ($ok\<acute>)"  "\<lceil>\<sigma>\<rceil>\<^sub>S\<^sub>A\<^sub>B\<^sub>R \<dagger> (\<not>$ok\<acute>) = (\<not>$ok\<acute>)"
   by (simp_all add: usubst unrest)
-
-lemma abrupt_ok_simpl[uabr_comp]:
-  "($abrupt;; Simpl\<^sub>A\<^sub>B\<^sub>R P) = $abrupt" "(\<not>$ok;; Simpl\<^sub>A\<^sub>B\<^sub>R P) = (\<not>$ok)"
+    
+lemma abrupt_simpl_axioms[uabr_comp]:
+  "($abrupt;; Simpl\<^sub>A\<^sub>B\<^sub>R (P \<turnstile> Q)) = $abrupt" "(\<not>$ok;; Simpl\<^sub>A\<^sub>B\<^sub>R (P \<turnstile> Q)) = (\<not>$ok)"
   "($abrupt;; (P \<turnstile> Q)) = $abrupt" "(\<not>$ok;; (P \<turnstile> Q)) = (\<not>$ok)"
-  "(\<not>$abrupt;; Simpl\<^sub>A\<^sub>B\<^sub>R P) = (\<not>$abrupt)" "(\<not>$ok;; Simpl\<^sub>A\<^sub>B\<^sub>R P) = (\<not>$ok)"
+  "(\<not>$abrupt;; Simpl\<^sub>A\<^sub>B\<^sub>R (P \<turnstile> Q)) = (\<not>$abrupt)" "(\<not>$ok;; Simpl\<^sub>A\<^sub>B\<^sub>R (P \<turnstile> Q)) = (\<not>$ok)"
   "(\<not>$abrupt;; (P \<turnstile> Q)) = (\<not>$abrupt)" "(\<not>$ok;; (P \<turnstile> Q)) = (\<not>$ok)"
   "($abrupt\<acute>;; Simpl\<^sub>A\<^sub>B\<^sub>R P) = $abrupt\<acute>"
   "(\<not>$abrupt\<acute>;; Simpl\<^sub>A\<^sub>B\<^sub>R P) = (\<not>$abrupt\<acute>)"
   by rel_auto+
 
 lemma simpl_abr_in_ok:
-  "Simpl\<^sub>A\<^sub>B\<^sub>R ($ok) = ((\<not>$abrupt \<and> ($ok \<Rightarrow>$ok\<acute>)) \<or> (II))"
+  "Simpl\<^sub>A\<^sub>B\<^sub>R ($ok) = ((\<not>$abrupt \<and> $ok ) \<or> ($abrupt \<and> II))"
   by rel_auto
 
 lemma  simpl_abr_our_ok:
   "Simpl\<^sub>A\<^sub>B\<^sub>R ($ok\<acute>) =
-   ((\<not>$abrupt \<and> ($ok \<Rightarrow>$ok\<acute>)) \<or> (II))"
+   ((\<not>$abrupt \<and> $ok\<acute>) \<or> ($abrupt \<and> II))"
   by rel_auto
 
 lemma simpl_abr_in_abrupt:
-  "Simpl\<^sub>A\<^sub>B\<^sub>R ($abrupt) =
-   ((\<not>$abrupt \<and> ($ok \<Rightarrow>($ok\<acute> \<and> $abrupt))) \<or> ($abrupt \<and> II))"
+  "Simpl\<^sub>A\<^sub>B\<^sub>R ($abrupt) =  ($abrupt \<and> II)"
   by rel_auto
 
 lemma simpl_abr_alr_def:
-  "Simpl\<^sub>A\<^sub>B\<^sub>R (P) =
-   ((\<not>$abrupt \<and> ($ok \<Rightarrow>($ok\<acute> \<and> P))) \<or> ($abrupt \<and> II))"
+  "Simpl\<^sub>A\<^sub>B\<^sub>R (P) = ((\<not>$abrupt \<and> P) \<or> ($abrupt \<and> II))"
   by rel_auto
     
 subsection \<open>Healthiness condition behavior\<close>
-
-lemma rel_usubst_cpa_c3_abr[usubst]:
-  assumes "$ok \<sharp> \<sigma>" "$ok\<acute> \<sharp> \<sigma> "
-  shows "\<sigma> \<dagger> C3_abr(P) = (\<sigma> \<dagger> P \<triangleleft> \<sigma> \<dagger> (\<not>$abrupt) \<triangleright> (\<sigma> \<dagger> II))"
-  using assms unfolding C3_abr_def
-  by (simp add: usubst)
 
 lemma Simpl_abr_idem[simp]: "Simpl\<^sub>A\<^sub>B\<^sub>R(Simpl\<^sub>A\<^sub>B\<^sub>R(P)) = Simpl\<^sub>A\<^sub>B\<^sub>R(P)"
   by (rel_auto)
@@ -109,37 +101,32 @@ lemma Simpl_abr_mono: "P \<sqsubseteq> Q \<Longrightarrow> Simpl\<^sub>A\<^sub>B
 lemma simpl_abr_Monotonic: "Monotonic Simpl\<^sub>A\<^sub>B\<^sub>R"
   by (simp add: mono_def Simpl_abr_mono)
 
-lemma simpl_abr_def:
-  "Simpl\<^sub>A\<^sub>B\<^sub>R(P) = ((\<lceil>true\<rceil>\<^sub>A\<^sub>B\<^sub>R \<turnstile> P) \<triangleleft> \<not>$abrupt \<triangleright>  II)"
-  unfolding C3_abr_def ..
-
-
 lemma simpl_abr_condr[uabr_simpl]:
   "Simpl\<^sub>A\<^sub>B\<^sub>R(P \<triangleleft> b \<triangleright> Q) = (Simpl\<^sub>A\<^sub>B\<^sub>R(P) \<triangleleft> b \<triangleright> Simpl\<^sub>A\<^sub>B\<^sub>R(Q))"
-  unfolding simpl_abr_def
   by (simp add: urel_cond)
-
+    
 lemma simpl_abr_skip_abr[uabr_simpl]:
   "Simpl\<^sub>A\<^sub>B\<^sub>R(SKIP\<^sub>A\<^sub>B\<^sub>R) = (SKIP\<^sub>A\<^sub>B\<^sub>R)"
-  by (simp add: urel_cond urel_defs)
+  by rel_auto
 
 lemma simpl_abr_throw_abr:
-  "Simpl\<^sub>A\<^sub>B\<^sub>R(THROW\<^sub>A\<^sub>B\<^sub>R) = ((\<not>$abrupt) \<and> ($ok \<Rightarrow>($ok\<acute> \<and> $abrupt\<acute> \<and> \<lceil>II\<rceil>\<^sub>A\<^sub>B\<^sub>R)) \<or> ($abrupt \<and> II))"
+  "Simpl\<^sub>A\<^sub>B\<^sub>R(THROW\<^sub>A\<^sub>B\<^sub>R) = ((\<not>$abrupt) \<and> ($ok \<Rightarrow> ($ok\<acute> \<and> $abrupt\<acute> \<and> \<lceil>II\<rceil>\<^sub>A\<^sub>B\<^sub>R)) \<or> ($abrupt \<and> II))"
   by rel_auto
 
 lemma simpl_abr_assign_abr[uabr_simpl]:
   "Simpl\<^sub>A\<^sub>B\<^sub>R(\<langle>\<sigma>\<rangle>\<^sub>A\<^sub>B\<^sub>R) = (\<langle>\<sigma>\<rangle>\<^sub>A\<^sub>B\<^sub>R)"
-  by (simp add: urel_cond urel_defs)
+  by rel_auto
 
 lemma simpl_abr_throw_abr_comp_abrupt[uabr_simpl]:
-  "Simpl\<^sub>A\<^sub>B\<^sub>R (THROW\<^sub>A\<^sub>B\<^sub>R;; ((abrupt :== (\<not> &abrupt);; Simpl\<^sub>A\<^sub>B\<^sub>R Q) \<triangleleft> $abrupt \<triangleright> II)) = Simpl\<^sub>A\<^sub>B\<^sub>R Q"
+  "Simpl\<^sub>A\<^sub>B\<^sub>R (THROW\<^sub>A\<^sub>B\<^sub>R;; ((abrupt :== (\<not> &abrupt);; Simpl\<^sub>A\<^sub>B\<^sub>R (P \<turnstile> Q)) \<triangleleft> $abrupt \<triangleright> II)) = 
+   Simpl\<^sub>A\<^sub>B\<^sub>R (P \<turnstile> Q)"
    apply pred_simp
    apply rel_simp
    apply auto
 done
 
 lemma simpl_abr_throw_abr_comp_abrupt_cond_throw_abr[uabr_simpl]:
-  "Simpl\<^sub>A\<^sub>B\<^sub>R (THROW\<^sub>A\<^sub>B\<^sub>R;; ((abrupt :== (\<not> &abrupt);; THROW\<^sub>A\<^sub>B\<^sub>R) \<triangleleft> $abrupt \<triangleright> II)) = Simpl\<^sub>A\<^sub>B\<^sub>R THROW\<^sub>A\<^sub>B\<^sub>R"
+  "Simpl\<^sub>A\<^sub>B\<^sub>R (THROW\<^sub>A\<^sub>B\<^sub>R;; ((abrupt :== (\<not> &abrupt);; THROW\<^sub>A\<^sub>B\<^sub>R) \<triangleleft> $abrupt \<triangleright> II)) = THROW\<^sub>A\<^sub>B\<^sub>R"
    apply pred_simp
    apply rel_simp
    apply auto
@@ -159,43 +146,7 @@ lemma simpl_abr_throw_abr_comp_abrupt_cond_assigns_abr[uabr_simpl]:
    apply auto
 done
 
-lemma C3_abr_throw_abr_comp_abrupt[uabr_simpl]:
-  "C3_abr (THROW\<^sub>A\<^sub>B\<^sub>R;; ((abrupt :== (\<not> &abrupt);; Simpl\<^sub>A\<^sub>B\<^sub>R Q) \<triangleleft> $abrupt \<triangleright> II)) =
-    Simpl\<^sub>A\<^sub>B\<^sub>R Q"
-  apply pred_simp
-  apply rel_simp
-  apply safe
-  apply auto
-done
-
-lemma C3_abr_throw_abr_comp_abrupt_cond_skip_abr[uabr_simpl]:
-  "C3_abr (THROW\<^sub>A\<^sub>B\<^sub>R;; ((abrupt :== (\<not> &abrupt);; SKIP\<^sub>A\<^sub>B\<^sub>R) \<triangleleft> $abrupt \<triangleright> II)) =
-    SKIP\<^sub>A\<^sub>B\<^sub>R"
-  apply pred_simp
-  apply rel_simp
-  apply safe
-  apply auto
-done
-
-lemma C3_abr_throw_abr_comp_abrupt_cond_throw_abr[uabr_simpl]:
-  "C3_abr (THROW\<^sub>A\<^sub>B\<^sub>R;; ((abrupt :== (\<not> &abrupt);; THROW\<^sub>A\<^sub>B\<^sub>R) \<triangleleft> $abrupt \<triangleright> II)) =
-    C3_abr THROW\<^sub>A\<^sub>B\<^sub>R"
-  apply pred_simp
-  apply rel_simp
-  apply safe
-  apply auto
-done
-
-lemma C3_abr_throw_abr_comp_abrupt_cond_assigns_abr[uabr_simpl]:
-  "C3_abr (THROW\<^sub>A\<^sub>B\<^sub>R;; ((abrupt :== (\<not> &abrupt);; \<langle>\<sigma>\<rangle>\<^sub>A\<^sub>B\<^sub>R) \<triangleleft> $abrupt \<triangleright> II)) =
-    \<langle>\<sigma>\<rangle>\<^sub>A\<^sub>B\<^sub>R"
-  apply pred_simp
-  apply rel_simp
-  apply safe
-  apply auto
-done
-
-(*lemma [uabr_comp]:
+lemma [uabr_comp]:
   "(THROW\<^sub>A\<^sub>B\<^sub>R;; ((abrupt :== (\<not> &abrupt);; THROW\<^sub>A\<^sub>B\<^sub>R) \<triangleleft> $abrupt \<triangleright> II)) =
    (\<lceil>true\<rceil>\<^sub>A\<^sub>B\<^sub>R \<turnstile> ($abrupt\<acute> \<and> \<lceil>II\<rceil>\<^sub>A\<^sub>B\<^sub>R)) "
   apply pred_simp
@@ -220,7 +171,7 @@ lemma [uabr_comp]:
   apply rel_simp
   apply safe
   apply auto
-done*)
+done
 
 lemma [uabr_comp]:
   "(THROW\<^sub>A\<^sub>B\<^sub>R;; ((abrupt :== (\<not> &abrupt);; \<lceil>true\<rceil>\<^sub>A\<^sub>B\<^sub>R) \<triangleleft> $abrupt \<triangleright> II)) = (true) "
@@ -230,7 +181,7 @@ lemma [uabr_comp]:
 done
 
 lemma simpl_abr_form:
-  "Simpl\<^sub>A\<^sub>B\<^sub>R(P) = (((\<not>$abrupt) \<and> (\<lceil>true\<rceil>\<^sub>A\<^sub>B\<^sub>R \<turnstile> (P)))  \<or> ($abrupt \<and> II))"
+  "Simpl\<^sub>A\<^sub>B\<^sub>R(P) = (((\<not>$abrupt) \<and> (P))  \<or> ($abrupt \<and> II))"
   by rel_auto
 
 lemma abrupt_simpl_abr[uabr_simpl]:
@@ -238,10 +189,10 @@ lemma abrupt_simpl_abr[uabr_simpl]:
    by rel_auto
 
 lemma nabrupt_simpl_abr[uabr_simpl]:
-  "(\<not>$abrupt \<and> Simpl\<^sub>A\<^sub>B\<^sub>R(P)) = (\<not>$abrupt \<and> (\<lceil>true\<rceil>\<^sub>A\<^sub>B\<^sub>R \<turnstile> (P)))"
+  "(\<not>$abrupt \<and> Simpl\<^sub>A\<^sub>B\<^sub>R(P)) = (\<not>$abrupt \<and> (P))"
   by (rel_auto)
 
-definition design_abr_sup :: "('\<alpha>,'\<beta>) rel_cpa set \<Rightarrow> ('\<alpha>,'\<beta>) rel_cpa" ("\<Sqinter>\<^sub>A\<^sub>B\<^sub>R_" [900] 900) where
+definition design_abr_sup :: "('\<alpha>,'\<beta>) rel_abr_des set \<Rightarrow> ('\<alpha>,'\<beta>) rel_abr_des" ("\<Sqinter>\<^sub>A\<^sub>B\<^sub>R_" [900] 900) where
 "\<Sqinter>\<^sub>A\<^sub>B\<^sub>R A = (if (A = {}) then \<top>\<^sub>A\<^sub>B\<^sub>R else \<Sqinter> A)"
 
 lemma simpl_abr_Continuous: 
@@ -275,7 +226,7 @@ lemma design_abr_sup_empty [simp]:
   "\<Sqinter>\<^sub>A\<^sub>B\<^sub>R {} = \<top>\<^sub>A\<^sub>B\<^sub>R"
   by (simp add: design_abr_sup_def)
 
-abbreviation design_inf :: "('\<alpha>, '\<beta>) rel_des set \<Rightarrow> ('\<alpha>, '\<beta>) rel_des" ("\<Squnion>\<^sub>A\<^sub>B\<^sub>R_" [900] 900) where
+abbreviation design_inf :: "('\<alpha>, '\<beta>) rel_abr_des set \<Rightarrow> ('\<alpha>, '\<beta>) rel_abr_des" ("\<Squnion>\<^sub>A\<^sub>B\<^sub>R_" [900] 900) where
   "\<Squnion>\<^sub>A\<^sub>B\<^sub>R A \<equiv> \<Squnion> A"
 
 lemma design_bottom_abr:
@@ -346,10 +297,10 @@ lemma usubst_cpa_skip_cpa [usubst]:
 lemma usubst_cpa_throw_cpa [usubst]:
   assumes "$ok \<sharp> \<sigma>" "$ok\<acute> \<sharp> \<sigma> "
   shows
-  "(\<sigma> \<dagger> THROW\<^sub>A\<^sub>B\<^sub>R) = (\<sigma> \<dagger> (\<not>$abrupt) \<turnstile> (\<sigma> \<dagger> ($abrupt\<acute> \<and> \<lceil>II\<rceil>\<^sub>A\<^sub>B\<^sub>R)))"
+  "(\<sigma> \<dagger> THROW\<^sub>A\<^sub>B\<^sub>R) = \<sigma> \<dagger> Simpl\<^sub>A\<^sub>B\<^sub>R ( \<lceil>true\<rceil>\<^sub>A\<^sub>B\<^sub>R \<turnstile> ($abrupt\<acute> \<and> \<lceil>II\<rceil>\<^sub>A\<^sub>B\<^sub>R))"
   using assms unfolding throw_abr_def
-  by (simp add: usubst)
-
+  by rel_auto
+    
 lemma usubst_cpa_assigns_cpa [usubst]:
   assumes "$ok \<sharp> \<sigma>" "$ok\<acute> \<sharp> \<sigma> "
   shows
@@ -357,23 +308,9 @@ lemma usubst_cpa_assigns_cpa [usubst]:
   using assms unfolding assigns_abr_def
   by (simp add: usubst)
 
-lemma simpl_comp_left_distr:
-  "(C3_abr (P);; R) = ((P;; R) \<triangleleft> \<not>$abrupt \<triangleright> (II;; R))"
-  apply pred_simp
-  apply rel_simp
-  apply fastforce
-done
-
-lemma c3_abr_comp_semir:
-  "(C3_abr(P);; C3_abr(R)) = C3_abr (P;; C3_abr(R))"
-  by rel_auto
-
-lemma c3_abr_comp_simpl[uabr_comp]:
-  "(C3_abr(P);; C3_abr(R)) = ((P;; C3_abr(R)) \<triangleleft> \<not>$abrupt \<triangleright> (II))"
-  by rel_auto
 
 lemma simpl_abr_comp_semir:
-  "(Simpl\<^sub>A\<^sub>B\<^sub>R(P);; Simpl\<^sub>A\<^sub>B\<^sub>R(R)) = Simpl\<^sub>A\<^sub>B\<^sub>R ((\<lceil>true\<rceil>\<^sub>A\<^sub>B\<^sub>R \<turnstile> P);; Simpl\<^sub>A\<^sub>B\<^sub>R(R))"
+  "(Simpl\<^sub>A\<^sub>B\<^sub>R(P);; Simpl\<^sub>A\<^sub>B\<^sub>R(R)) = Simpl\<^sub>A\<^sub>B\<^sub>R (P;; Simpl\<^sub>A\<^sub>B\<^sub>R(R))"
   by rel_auto
 
 theorem design_top_abr_left_zero[uabr_comp]:
@@ -381,7 +318,7 @@ theorem design_top_abr_left_zero[uabr_comp]:
   by (rel_auto)
 
 theorem Simpl_abr_top_abr_left_zero[uabr_comp]:
-  "(\<top>\<^sub>A\<^sub>B\<^sub>R;; Simpl\<^sub>A\<^sub>B\<^sub>R (P)) = \<top>\<^sub>A\<^sub>B\<^sub>R"
+  "(\<top>\<^sub>A\<^sub>B\<^sub>R;; Simpl\<^sub>A\<^sub>B\<^sub>R (P)) = (\<top>\<^sub>A\<^sub>B\<^sub>R ;; ((\<not>$abrupt  \<and> P) \<or> ($abrupt \<and> II)))"
   by (rel_auto)
 
 lemma assigns_lift_cpa_comp_rel_cpa[uabr_comp]:
@@ -398,14 +335,22 @@ lemma lift_des_skip_dr_unit_abr[uabr_comp]:
   by (rel_auto)+
 
 lemma skip_cpa_left_comp_simpl[uabr_comp]:
-  "(SKIP\<^sub>A\<^sub>B\<^sub>R;; Simpl\<^sub>A\<^sub>B\<^sub>R(R)) = (Simpl\<^sub>A\<^sub>B\<^sub>R(R))"
+  "(SKIP\<^sub>A\<^sub>B\<^sub>R;; Simpl\<^sub>A\<^sub>B\<^sub>R(P \<turnstile> Q)) = (Simpl\<^sub>A\<^sub>B\<^sub>R(P \<turnstile> Q))"
   by rel_auto
-
+    
+lemma "(Simpl\<^sub>A\<^sub>B\<^sub>R (\<lceil>P\<rceil>\<^sub>A\<^sub>B\<^sub>R \<turnstile> (\<lceil>Q\<rceil>\<^sub>A\<^sub>B\<^sub>R)) ;; SKIP\<^sub>A\<^sub>B\<^sub>R) = (Simpl\<^sub>A\<^sub>B\<^sub>R (\<lceil>P\<rceil>\<^sub>A\<^sub>B\<^sub>R \<turnstile> (\<lceil>Q\<rceil>\<^sub>A\<^sub>B\<^sub>R)))"
+  apply pred_simp
+  apply rel_simp
+  apply auto  
+  apply auto 
+    
+    
+    (**
 lemma skip_cpa_right_comp_simpl[uabr_comp]:
-  "(Simpl\<^sub>A\<^sub>B\<^sub>R(R);; SKIP\<^sub>A\<^sub>B\<^sub>R) = (Simpl\<^sub>A\<^sub>B\<^sub>R(R))"
+  "(Simpl\<^sub>A\<^sub>B\<^sub>R (P \<turnstile> Q);; SKIP\<^sub>A\<^sub>B\<^sub>R) = Simpl\<^sub>A\<^sub>B\<^sub>R  ((P \<turnstile> Q) ;; SKIP\<^sub>A\<^sub>B\<^sub>R)"
   by rel_auto
 
-lemma throw_cpa_left_comp_simpl[uabr_comp]:
+lemma throw_abr_left_zero_simpl_abr[uabr_comp]:
   "(THROW\<^sub>A\<^sub>B\<^sub>R;; Simpl\<^sub>A\<^sub>B\<^sub>R(R)) = (THROW\<^sub>A\<^sub>B\<^sub>R)"
   by rel_auto
 
@@ -413,9 +358,6 @@ lemma assign_abr_alt_def:
   "\<langle>\<sigma>\<rangle>\<^sub>A\<^sub>B\<^sub>R = Simpl\<^sub>A\<^sub>B\<^sub>R (\<not>$abrupt\<acute> \<and> \<lceil>\<lceil>\<sigma>\<rceil>\<^sub>s \<dagger> II\<rceil>\<^sub>A\<^sub>B\<^sub>R)"
   by rel_auto
 
-lemma assign_abr_left_comp_c3[uabr_comp]:
-  "\<langle>a\<rangle>\<^sub>A\<^sub>B\<^sub>R;; C3_abr (P \<turnstile> Q) = C3_abr (\<lceil>a\<rceil>\<^sub>s\<^sub>A\<^sub>B\<^sub>R \<dagger> (P \<turnstile> Q))"
-  by rel_auto
 
 lemma assigns_abr_comp[uabr_comp]:
   "(\<langle>f\<rangle>\<^sub>A\<^sub>B\<^sub>R;; \<langle>g\<rangle>\<^sub>A\<^sub>B\<^sub>R) = \<langle>g \<circ> f\<rangle>\<^sub>A\<^sub>B\<^sub>R"
@@ -423,21 +365,20 @@ lemma assigns_abr_comp[uabr_comp]:
 
 lemma usubst_cpa_des_cond_abr[usubst]:
   "\<lbrakk> $ok \<sharp> \<sigma>; $ok\<acute> \<sharp> \<sigma> \<rbrakk> \<Longrightarrow>
-    \<sigma> \<dagger> (R \<turnstile> bif b then P else Q eif) =
-    (\<sigma> \<dagger> R \<turnstile> (\<sigma> \<dagger> P \<triangleleft> \<sigma> \<dagger> \<lceil>b\<rceil>\<^sub>A\<^sub>B\<^sub>R\<^sub>< \<triangleright> \<sigma> \<dagger> Q))"
+    (\<sigma> \<dagger> (R \<turnstile> (bif\<^sub>A\<^sub>B\<^sub>R b then P else Q eif))) =
+    ((\<sigma> \<dagger> R) \<turnstile> (\<sigma> \<dagger> Simpl\<^sub>A\<^sub>B\<^sub>R( P \<triangleleft> \<lceil>b\<rceil>\<^sub>A\<^sub>B\<^sub>R\<^sub>< \<triangleright>  Q)))"
   by (simp add: usubst)
 
+
 lemma comp_cond_abr_left_distr[uabr_comp]:
-  "((bif b then Simpl\<^sub>A\<^sub>B\<^sub>R P else Simpl\<^sub>A\<^sub>B\<^sub>R Q eif);; Simpl\<^sub>A\<^sub>B\<^sub>R R) =
-    (bif b then (Simpl\<^sub>A\<^sub>B\<^sub>R P;; Simpl\<^sub>A\<^sub>B\<^sub>R R) else (Simpl\<^sub>A\<^sub>B\<^sub>R Q;; Simpl\<^sub>A\<^sub>B\<^sub>R R) eif)"
-  apply (simp add: usubst uabr_comp)
+  "((bif\<^sub>A\<^sub>B\<^sub>R b then Simpl\<^sub>A\<^sub>B\<^sub>R P else Simpl\<^sub>A\<^sub>B\<^sub>R Q eif);; Simpl\<^sub>A\<^sub>B\<^sub>R R) =
+    (bif\<^sub>A\<^sub>B\<^sub>R b then (Simpl\<^sub>A\<^sub>B\<^sub>R P;; Simpl\<^sub>A\<^sub>B\<^sub>R R) else (Simpl\<^sub>A\<^sub>B\<^sub>R Q;; Simpl\<^sub>A\<^sub>B\<^sub>R R) eif)"
   apply pred_simp
-  apply rel_simp
-  apply auto
+  apply rel_auto  
 done
 
 lemma if_mono:
-  "\<lbrakk> P\<^sub>1 \<sqsubseteq> P\<^sub>2; Q\<^sub>1 \<sqsubseteq> Q\<^sub>2 \<rbrakk> \<Longrightarrow> (bif b then P\<^sub>1 else Q\<^sub>1 eif) \<sqsubseteq> (bif b then P\<^sub>2 else Q\<^sub>2 eif)"
+  "\<lbrakk> P\<^sub>1 \<sqsubseteq> P\<^sub>2; Q\<^sub>1 \<sqsubseteq> Q\<^sub>2 \<rbrakk> \<Longrightarrow> (bif\<^sub>A\<^sub>B\<^sub>R b then P\<^sub>1 else Q\<^sub>1 eif) \<sqsubseteq> (bif\<^sub>A\<^sub>B\<^sub>R b then P\<^sub>2 else Q\<^sub>2 eif)"
   by rel_auto
 
 subsection \<open>While abrupt usubst\<close>
