C-verifier/src/Midend-IVL/Isabelle-UTP/impl/utp_prog.thy
@@ -39,8 +39,8 @@ method ptransfer = (simp add: prog_rep_eq)
     
 subsection {* Operators *}
   
-lift_definition abort    :: "'\<alpha> prog" is "true" by (simp add: closure)
-lift_definition magic    :: "'\<alpha> prog" is "\<top>\<^sub>D" by (simp add: closure)
+lift_definition abort    :: "'\<alpha> prog" ("ABORT") is "true" by (simp add: closure)
+lift_definition magic    :: "'\<alpha> prog" ("MAGIC") is "\<top>\<^sub>D" by (simp add: closure)
 lift_definition skip     :: "'\<alpha> prog" ("SKIP")is "II\<^sub>D" by (simp add: closure)
 lift_definition pseq     :: "'\<alpha> prog \<Rightarrow> '\<alpha> prog \<Rightarrow> '\<alpha> prog" (infix ";" 71) is "op ;;" by (simp add: closure)
 lift_definition passigns :: "'\<alpha> usubst \<Rightarrow> '\<alpha> prog" ("\<langle>_\<rangle>\<^sub>p") is "assigns_d" by (simp add: closure)
